lib/corres_method: method for corres_rv
This removes corres_choice in favour of making corres_rv smarter.
Now corres_rv can propagate a stateless condition, and the new
corres_rv method (called from corres) tries to push the generated
obligation into the appropriate place (stateless, left or right
precondition) based on which variables it discusses.

This avoids most cases where the corres_rv_wp_left/right or
corres_rv_defer rules needed to be specified manually.

lib/Corres_Method.thy
@@ -84,41 +84,6 @@ lemma corresK_lift_rule:
 
 lemmas corresK_drop = corresK_drop_any_guard[where F=True]
 
-definition
-  "corres_choice_true B P \<equiv>
-    B \<longrightarrow> P"
-
-lemma corres_choice_trueD:
-  "corres_choice_true B P \<Longrightarrow> B  \<Longrightarrow> P" by (simp add: corres_choice_true_def)
-
-lemma corres_choice_true_simps[simp]:
-  "corres_choice_true True P = P"
-  "corres_choice_true False P = True"
-  by (simp add: corres_choice_true_def)+
-
-lemma corres_choice_true_True:
-  "P \<Longrightarrow> corres_choice_true True P" by (simp)
-
-definition
-  "corres_choice_false B P \<equiv>
-    (\<not> B) \<longrightarrow> P"
-
-lemma corres_choice_false_simps[simp]:
-  "corres_choice_false False P = P"
-  "corres_choice_false True P = True"
-  by (simp add: corres_choice_false_def)+
-
-lemma corres_choice_falseD:
-  "corres_choice_false B P \<Longrightarrow> \<not> B \<Longrightarrow> P" by (simp add: corres_choice_false_def)
-
-lemma corres_choice_rv[wp]:
-  "\<lbrace>RR\<rbrace> m \<lbrace>\<lambda>rv s. F rv\<rbrace> \<Longrightarrow> corres_choice_true True (\<lbrace>RR\<rbrace> m \<lbrace>\<lambda>rv s. F rv\<rbrace>)"
-  by simp
-
-lemma corres_choice_no_rv[wp]:
-  "corres_choice_true False (\<lbrace>\<lambda>_. True\<rbrace> m \<lbrace>\<lambda>_ _. F\<rbrace>)"
-  by simp
-
 context begin
 
 lemma corresK_start:
@@ -366,70 +331,181 @@ text \<open>
  of the refinement.
  \<close>
 
-definition corres_rv ::"(('s \<times> 't) set) \<Rightarrow>
-                        ('a \<Rightarrow> 'b \<Rightarrow> bool) \<Rightarrow> ('s \<Rightarrow> bool) \<Rightarrow> ('t \<Rightarrow> bool)
-           \<Rightarrow> ('s, 'a) nondet_monad \<Rightarrow> ('t, 'b) nondet_monad \<Rightarrow> bool"
+definition "corres_noop = return undefined"
+
+definition corres_rv :: "bool \<Rightarrow> ('a \<Rightarrow> 'b \<Rightarrow> bool) \<Rightarrow> ('s \<Rightarrow> bool) \<Rightarrow> ('t \<Rightarrow> bool)
+           \<Rightarrow> ('s, 'a) nondet_monad \<Rightarrow> ('t, 'b) nondet_monad \<Rightarrow>
+            ('a \<Rightarrow> 'b \<Rightarrow> bool) \<Rightarrow> bool"
   where
-  "corres_rv sr r P P' f f' \<equiv>
-   \<forall>(s,s') \<in> sr. P s \<longrightarrow> P' s' \<longrightarrow>
-    (\<forall>sa rv. (rv, sa) \<in> fst (f s) \<longrightarrow> (\<forall>sa' rv'. (rv', sa') \<in> fst (f' s') \<longrightarrow> (sa,sa') \<in> sr \<longrightarrow> r rv rv'))"
+  "corres_rv F r P P' f f' Q \<equiv>
+   F \<longrightarrow> (\<forall>s s'. P s \<longrightarrow> P' s' \<longrightarrow>
+    (\<forall>sa rv. (rv, sa) \<in> fst (f s) \<longrightarrow> (\<forall>sa' rv'. (rv', sa') \<in> fst (f' s') \<longrightarrow> r rv rv' \<longrightarrow> Q rv rv')))"
+
+
+definition "corres_rvE_R F r P P' f f' Q \<equiv>
+  corres_rv F (\<lambda>_ _. True) P P' f f'
+    (\<lambda>rvE rvE'. case (rvE,rvE') of (Inr rv, Inr rv') \<Rightarrow> r rv rv' \<longrightarrow> Q rv rv' | _ \<Rightarrow> True)"
 
 lemma corres_rvD:
-  "corres_rv sr r P P' f f' \<Longrightarrow>
-   (s,s') \<in> sr \<Longrightarrow> P s \<Longrightarrow> P' s' \<Longrightarrow> (rv,sa) \<in> fst (f s) \<Longrightarrow>
-      (rv',sa') \<in> fst (f' s') \<Longrightarrow> (sa,sa') \<in> sr \<Longrightarrow> r rv rv'"
+  "corres_rv F r P P' f f' Q \<Longrightarrow>
+   F \<Longrightarrow> P s \<Longrightarrow> P' s' \<Longrightarrow> (rv,sa) \<in> fst (f s) \<Longrightarrow>
+      (rv',sa') \<in> fst (f' s') \<Longrightarrow> r rv rv' \<Longrightarrow> Q rv rv'"
   by (auto simp add: corres_rv_def)
+
+lemma corres_rvE_RD:
+  "corres_rvE_R F r P P' f f' Q \<Longrightarrow>
+   F \<Longrightarrow> P s \<Longrightarrow> P' s' \<Longrightarrow> (Inr rv,sa) \<in> fst (f s) \<Longrightarrow>
+      (Inr rv',sa') \<in> fst (f' s') \<Longrightarrow> r rv rv' \<Longrightarrow> Q rv rv'"
+  by (auto simp add: corres_rv_def corres_rvE_R_def split: sum.splits)
+
+lemma corres_rv_cong[cong]:
+  "\<lbrakk>F = F'; r = r'; P = P'; PP = PP'; f = f'; g = g'; (\<And>rv rv'. r' rv rv' \<Longrightarrow> Q rv rv' = Q' rv rv')\<rbrakk> \<Longrightarrow>
+      corres_rv F r P PP f g Q = corres_rv F' r' P' PP' f' g' Q'"
+  by (simp add: corres_rv_def)
+
+lemma corres_rvE_R_cong[cong]:
+  "\<lbrakk>F = F'; r = r'; P = P'; PP = PP'; f = f'; g = g'; (\<And>rv rv'. r' rv rv' \<Longrightarrow> Q rv rv' = Q' rv rv')\<rbrakk> \<Longrightarrow>
+      corres_rvE_R F r P PP f g Q = corres_rvE_R F' r' P' PP' f' g' Q'"
+  by (auto simp add: corres_rv_def corres_rvE_R_def split: sum.splits)
 
 (* Working with corres_rv is not immediately intuitive, but most of the time it just goes away.
    Might need more rules if complex goals show up. *)
 
-lemma corres_rv_prove_raw:
-  "(\<And>s s' sa sa' rv rv'. (s,s') \<in> sr \<Longrightarrow> (sa,sa') \<in> sr \<Longrightarrow>
-    (rv,sa) \<in> fst (f s) \<Longrightarrow> (rv',sa') \<in> fst (f' s') \<Longrightarrow> P s \<Longrightarrow> P' s' \<Longrightarrow> r rv rv') \<Longrightarrow>
-    corres_rv sr r P P' f f'"
+lemma corres_rv_prove:
+  "(\<And>s s' sa sa' rv rv'. F \<Longrightarrow>
+    (rv,sa) \<in> fst (f s) \<Longrightarrow> (rv',sa') \<in> fst (f' s') \<Longrightarrow> P s \<Longrightarrow> P' s' \<Longrightarrow> r rv rv' \<Longrightarrow> Q rv rv') \<Longrightarrow>
+    corres_rv F r P P' f f' Q"
   by (auto simp add: corres_rv_def)
+
+lemma corres_rvE_R_prove:
+  "(\<And>s s' sa sa' rv rv'. F \<Longrightarrow>
+    (Inr rv,sa) \<in> fst (f s) \<Longrightarrow> (Inr rv',sa') \<in> fst (f' s') \<Longrightarrow> P s \<Longrightarrow> P' s' \<Longrightarrow> r rv rv' \<Longrightarrow> Q rv rv') \<Longrightarrow>
+    corres_rvE_R F r P P' f f' Q"
+  by (auto simp add: corres_rv_def corres_rvE_R_def split: sum.splits)
 
 lemma corres_rv_wp_left:
-  "\<lbrace>P\<rbrace> f \<lbrace>\<lambda>rv s. \<forall>rv'. r rv rv'\<rbrace> \<Longrightarrow> corres_choice_true True (corres_rv sr r P \<top> f f')"
+  "\<lbrace>P\<rbrace> f \<lbrace>\<lambda>rv s. \<forall>rv'. r rv rv' \<longrightarrow> Q rv rv'\<rbrace> \<Longrightarrow> corres_rv True r P \<top> f f' Q"
   by (fastforce simp add: corres_rv_def valid_def)
+
+lemma corres_rvE_R_wp_left:
+  "\<lbrace>P\<rbrace> f \<lbrace>\<lambda>rv s. \<forall>rv'. r rv rv' \<longrightarrow> Q rv rv'\<rbrace>, - \<Longrightarrow> corres_rvE_R True r P \<top> f f' Q"
+  apply (simp add: corres_rvE_R_def validE_def validE_R_def)
+  apply (rule corres_rv_wp_left)
+  apply (erule hoare_strengthen_post)
+  apply (auto split: sum.splits)
+  done
 
 lemma corres_rv_wp_right:
-  "\<lbrace>P'\<rbrace> f' \<lbrace>\<lambda>rv' s. \<forall>rv. r rv rv'\<rbrace> \<Longrightarrow> corres_choice_true True (corres_rv sr r \<top> P' f f')"
+  "\<lbrace>P'\<rbrace> f' \<lbrace>\<lambda>rv' s. \<forall>rv. r rv rv' \<longrightarrow> Q rv rv'\<rbrace> \<Longrightarrow> corres_rv True r \<top> P' f f' Q"
   by (fastforce simp add: corres_rv_def valid_def)
 
+lemma corres_rvE_R_wp_right:
+  "\<lbrace>P'\<rbrace> f' \<lbrace>\<lambda>rv' s. \<forall>rv. r rv rv' \<longrightarrow> Q rv rv'\<rbrace>, - \<Longrightarrow> corres_rvE_R True r \<top> P' f f' Q"
+  apply (simp add: corres_rvE_R_def validE_def validE_R_def)
+  apply (rule corres_rv_wp_right)
+  apply (erule hoare_strengthen_post)
+  apply (auto split: sum.splits)
+  done
+
 lemma corres_rv_weaken:
-  "(\<And>rv rv'. r rv rv' \<Longrightarrow> r' rv rv') \<Longrightarrow> corres_rv sr r P P' f f' \<Longrightarrow> corres_rv sr r' P P' f f'"
+  "(\<And>rv rv'. Q rv rv' \<Longrightarrow> Q' rv rv') \<Longrightarrow> corres_rv F r P P' f f' Q \<Longrightarrow> corres_rv F r P P' f f' Q'"
   by (auto simp add: corres_rv_def)
 
-lemma corres_choice_rv_defer_no_args[wp]:
-  "corres_choice_true False (corres_rv sr (\<lambda>_ _. F) (\<lambda>_. True) (\<lambda>_. True) f f')"
-  by simp
+lemma corres_rvE_R_weaken:
+  "(\<And>rv rv'. Q rv rv' \<Longrightarrow> Q' rv rv') \<Longrightarrow> corres_rvE_R F r P P' f f' Q \<Longrightarrow> corres_rvE_R F r P P' f f' Q'"
+  by (auto simp add: corres_rv_def corres_rvE_R_def split: sum.splits)
+
+lemma corres_rv_defer_no_args:
+  "corres_rv (\<forall>rv rv'. r rv rv' \<longrightarrow> F) r (\<lambda>_. True) (\<lambda>_. True) f f' (\<lambda>_ _. F)"
+  by (auto simp add: corres_rv_def)
+
+lemma corres_rvE_R_defer_no_args:
+  "corres_rvE_R (\<forall>rv rv'. r rv rv' \<longrightarrow> F) r (\<lambda>_. True) (\<lambda>_. True) f f' (\<lambda>_ _. F)"
+  by (auto simp add: corres_rv_def corres_rvE_R_def split: sum.splits)
 
 lemma corres_rv_defer:
-  "corres_choice_true False (corres_rv sr F (\<lambda>_. True) (\<lambda>_. True) f f')"
-  by simp
+  "corres_rv (\<forall>rv rv'. r rv rv' \<longrightarrow> Q rv rv') r (\<lambda>_. True) (\<lambda>_. True) f f' Q"
+  by (auto simp add: corres_rv_def)
 
-lemmas corres_rv_prove = corres_rv_prove_raw[THEN corres_choice_true_True]
+lemma corres_rvE_R_defer:
+  "corres_rvE_R (\<forall>rv rv'. r rv rv' \<longrightarrow> Q rv rv') r (\<lambda>_. True) (\<lambda>_. True) f f' Q"
+  by (auto simp add: corres_rv_def corres_rvE_R_def split: sum.splits)
 
 lemmas corres_rv_proveT =
-  corres_rv_prove[where P=\<top> and P'=\<top>, # \<open>simp\<close>]
+  corres_rv_prove[where P=\<top> and P'=\<top> and F=True, # \<open>simp\<close>]
 
 lemmas corres_rv_trivial[intro!, wp] =
-  corres_rv_prove[where r="\<lambda>_ _. True" and P=\<top> and P'=\<top>, OF TrueI]
+  corres_rv_prove[where Q="\<lambda>_ _. True" and P=\<top> and P'=\<top> and F=True, OF TrueI]
+
+lemmas corres_rvE_R_proveT =
+  corres_rvE_R_prove[where P=\<top> and P'=\<top> and F=True, # \<open>simp\<close>]
+
+lemmas corres_rvE_R_trivial[intro!, wp] =
+  corres_rvE_R_prove[where r="\<lambda>_ _. True" and P=\<top> and P'=\<top> and F=True, OF TrueI]
+
+lemma corres_rv_conj_lift:
+  "corres_rv F r P PP f g Q \<Longrightarrow> corres_rv F' r P' PP' f g Q' \<Longrightarrow>
+    corres_rv (F \<and> F') r (\<lambda>s. P s \<and> P' s) (\<lambda>s'. PP s' \<and> PP' s') f g (\<lambda>rv rv'. Q rv rv' \<and> Q' rv rv')"
+   by (clarsimp simp add: corres_rv_def)
+
+lemma corres_rvE_R_conj_lift:
+  "corres_rvE_R F r P PP f g Q \<Longrightarrow> corres_rvE_R F' r P' PP' f g Q' \<Longrightarrow>
+    corres_rvE_R (F \<and> F') r (\<lambda>s. P s \<and> P' s) (\<lambda>s'. PP s' \<and> PP' s') f g (\<lambda>rv rv'. Q rv rv' \<and> Q' rv rv')"
+   by (auto simp add: corres_rv_def corres_rvE_R_def split: sum.splits)
+
+context begin
+
+private lemma corres_rv_defer_left:
+  "corres_rv F r (\<lambda>_. \<forall>rv rv'. Q rv rv') P' f f' Q"
+  by (simp add: corres_rv_def)
+
+private lemma corres_rvE_R_defer_left:
+  "corres_rvE_R F r (\<lambda>_. \<forall>rv rv'. Q rv rv') P' f f' Q"
+  by (simp add: corres_rv_def corres_rvE_R_def split: sum.splits)
+
+private lemma corres_rv_defer_right:
+  "corres_rv F r P (\<lambda>_. \<forall>rv rv'. Q rv rv') f f' Q"
+  by (simp add: corres_rv_def)
+
+private lemma corres_rvE_R_defer_right:
+  "corres_rvE_R F r P (\<lambda>_. \<forall>rv rv'. Q rv rv') f f' Q"
+  by (simp add: corres_rv_def corres_rvE_R_def split: sum.splits)
+
+lemmas corres_noop_wp_left[where f'=corres_noop] = corres_rv_wp_left corres_rvE_R_wp_left
+lemmas corres_noop_wp_right[where f=corres_noop] = corres_rv_wp_right corres_rvE_R_wp_right
+
+named_theorems corres_rv_defers
+
+lemmas [corres_rv_defers] =
+  corres_rv_defer_no_args corres_rvE_R_defer_no_args
+
+named_theorems corres_rv_lifts
+
+lemmas [corres_rv_lifts] =
+  corres_rv_conj_lift corres_rvE_R_conj_lift
+
+method corres_rv declares corres_rv_defers =
+  ((rule corres_rv_defers corres_noop_wp_left corres_noop_wp_right |
+   (succeeds \<open>rule corres_rv_defer_left corres_rvE_R_defer_left\<close>,
+    rule corres_rv_wp_left corres_rvE_R_wp_left) |
+   (succeeds \<open>rule corres_rv_defer_right corres_rvE_R_defer_right\<close>,
+    rule corres_rv_wp_right corres_rvE_R_wp_right) |
+    rule corres_rv_lifts)+)[1]
+
+end
 
 lemma corresK_split:
   assumes x: "corres_underlyingK sr nf nf' F r' P P' a c"
   assumes y: "\<And>rv rv'. corres_protect (r' rv rv') \<Longrightarrow> corres_underlyingK sr nf nf' (F' rv rv') r (R rv) (R' rv') (b rv) (d rv')"
+  assumes c: "corres_rv F'' r' PP PP' a c F'"
   assumes z: "\<lbrace>Q\<rbrace> a \<lbrace>R\<rbrace>" "\<lbrace>Q'\<rbrace> c \<lbrace>R'\<rbrace>"
-  assumes c: "corres_choice_true B (corres_rv sr (\<lambda>rv rv'. r' rv rv' \<longrightarrow> F' rv rv') PP PP' a c)"
-  shows      "corres_underlyingK sr nf nf' (F \<and> (corres_choice_false B (\<forall>rv rv'. r' rv rv' \<longrightarrow> F' rv rv'))) r (PP and P and Q) (PP' and P' and Q') (a >>= (\<lambda>rv. b rv)) (c >>= (\<lambda>rv'. d rv'))"
+  shows      "corres_underlyingK sr nf nf' (F \<and> F'') r (PP and P and Q) (PP' and P' and Q') (a >>= (\<lambda>rv. b rv)) (c >>= (\<lambda>rv'. d rv'))"
   apply (clarsimp simp: corres_underlying_def corres_underlyingK_def bind_def)
   apply (rule conjI)
    apply (frule (3) x[simplified corres_underlyingK_def, rule_format, THEN corres_underlyingD],simp)
    apply clarsimp
    apply (drule(1) bspec,clarsimp)
-   apply (insert c;simp?)
-   apply (subgoal_tac "F' ac aaa")
+   apply (drule (5) corres_rvD[OF c])
    apply (rule_tac x="(ac,bc)" in bexI,clarsimp)
     apply (frule_tac s'=baa in y[simplified corres_underlyingK_def corres_protect_def, rule_format, THEN corres_underlyingD])
           apply assumption+
@@ -439,30 +515,16 @@ lemma corresK_split:
     apply clarsimp
     apply (drule(1) bspec,clarsimp)
    apply simp
-  apply (cases B)
-    apply (drule(1) corres_choice_trueD)
-       apply (drule(6) corres_rvD)
-    apply clarsimp
-    apply (drule(1) corres_choice_falseD)
-    apply clarsimp
-  apply clarsimp
   apply (frule (3) x[simplified corres_underlyingK_def, rule_format, THEN corres_underlyingD],simp)
   apply clarsimp
   apply (drule(1) bspec,clarsimp)
-  apply (insert c;simp?)
-  apply (subgoal_tac "F' ab aaa")
+  apply (drule (5) corres_rvD[OF c])
   apply (frule_tac s'=baa in y[simplified corres_underlyingK_def corres_protect_def, rule_format, THEN corres_underlyingD])
         apply simp+
      apply (erule(1) use_valid[OF _ z(1)])
     apply (erule(1) use_valid[OF _ z(2)])
    apply fastforce
   apply clarsimp
-      apply (cases B)
-    apply (drule(1) corres_choice_trueD)
-       apply (drule(6) corres_rvD)
-    apply clarsimp
-    apply (drule(1) corres_choice_falseD)
-    apply clarsimp
   done
 
 section \<open>Corres_inst\<close>
@@ -474,20 +536,15 @@ text \<open>Handles rare in-place subgoals generated by corres rules which need 
 
 definition "corres_inst_eq x y \<equiv> x = y"
 
-lemma corres_inst_eqI: "corres_inst_eq x x" by (simp add: corres_inst_eq_def)
+lemma corres_inst_eqI[wp]: "corres_inst_eq x x" by (simp add: corres_inst_eq_def)
 
 lemma corres_inst_test: "False \<Longrightarrow> corres_inst_eq x y" by simp
-
-named_theorems corres_inst_simp
 
 method corres_inst =
   (succeeds \<open>rule corres_inst_test\<close>, fails \<open>rule TrueI\<close>,
     (rule corres_inst_eqI |
       (clarsimp simp: corres_protect_def, rule corres_inst_eqI)
-     | (clarsimp simp: corres_protect_def corres_inst_simp, fastforce intro!: corres_inst_eqI)))[1]
-
-lemmas [corres_inst_simp] =
-  o_def inv_def
+     | (clarsimp simp: corres_protect_def, fastforce intro!: corres_inst_eqI)))[1]
 
 section \<open>Corres Method\<close>
 
@@ -540,7 +597,7 @@ private method corres_apply =
      #break "corres_apply",
    ((focus_concl \<open>(atomize (full))?\<close>, erule guard_collect, rule has_guard) | rule no_guard))[1]
 
-private method corres_alternate = corres_inst
+private method corres_alternate = corres_inst | corres_rv
 
 method corres_once declares corres_splits corres corresK corresc_simp =
    (corres_alternate |
@@ -645,40 +702,21 @@ lemma corresK_symb_exec_l_search[corres_symb_exec_ls]:
   fixes x :: "'b \<Rightarrow> 'a \<Rightarrow> ('d \<times> 'a) set \<times> bool"
   shows
   "\<lbrakk>\<And>s. \<lbrace>PP s\<rbrace> m \<lbrace>\<lambda>_. op = s\<rbrace>; \<And>rv. corres_underlyingK sr nf True (F rv) r (Q rv) P' (x rv) y;
-   empty_fail m; no_fail P m; \<lbrace>R\<rbrace> m \<lbrace>Q\<rbrace>; corres_choice_true B (\<lbrace>RR\<rbrace> m \<lbrace>\<lambda>rv s. F rv\<rbrace>)\<rbrakk>
-\<Longrightarrow> corres_underlyingK sr nf True (corres_choice_false B (\<forall>rv. F rv)) r (RR and P and R and (\<lambda>s. \<forall>s'. s = s' \<longrightarrow> PP s' s)) P' (m >>= x) y"
+   empty_fail m; no_fail P m; \<lbrace>R\<rbrace> m \<lbrace>Q\<rbrace>; corres_rv F' dc RR (\<lambda>_. True) m (corres_noop) (\<lambda>rv _. F rv)\<rbrakk>
+\<Longrightarrow> corres_underlyingK sr nf True F' r (RR and P and R and (\<lambda>s. \<forall>s'. s = s' \<longrightarrow> PP s' s)) P' (m >>= x) y"
   apply (clarsimp simp add: corres_underlyingK_def)
   apply (rule corres_name_pre)
-  apply (clarsimp simp: corres_underlying_def corres_underlyingK_def corres_choice_true_def
-                        corres_choice_false_def
+  apply (clarsimp simp: corres_underlying_def corres_underlyingK_def corres_noop_def
                         bind_def valid_def empty_fail_def no_fail_def)
-  apply (cases B; simp)
   apply (drule_tac x=a in meta_spec)+
   apply (drule_tac x=a in spec)+
   apply (drule mp, assumption)+
-
   apply (clarsimp simp: not_empty_eq)
+  apply (drule corres_rvD; (assumption | simp add: return_def)?)
   apply (drule_tac x="(aa,ba)" in bspec,simp)+
   apply clarsimp
   apply (drule_tac x=aa in meta_spec)
   apply clarsimp
-  apply (drule_tac x="(ba,b)" in bspec,simp)
-  apply clarsimp
-  apply (drule mp, fastforce)
-  apply clarsimp
-  apply (drule_tac x="(a,bb)" in bspec,simp)
-  apply clarsimp
-  apply (rule_tac x="(aa,ba)" in bexI)
-   apply (clarsimp)
-   apply (rule_tac x="(ab,bc)" in bexI)
-    apply (clarsimp)+
-   apply (drule_tac x=a in meta_spec)+
-  apply (drule_tac x=a in spec)+
-  apply (drule mp, assumption)+
-  apply (clarsimp simp: not_empty_eq)
-  apply (drule_tac x="(aa,ba)" in bspec,simp)+
-  apply clarsimp
-  apply (drule_tac x=aa in meta_spec)
   apply (drule_tac x="(ba,b)" in bspec,simp)
   apply clarsimp
   apply (drule mp, fastforce)
@@ -701,9 +739,10 @@ lemma corresK_symb_exec_r_search[corres_symb_exec_rs]:
   assumes corres: "\<And>rv. corres_underlyingK sr nf nf' (F rv) r P (Q' rv) x (y rv)"
   assumes nf: "nf' \<Longrightarrow> no_fail P' m"
   assumes Z: "\<lbrace>R\<rbrace> m \<lbrace>Q'\<rbrace>"
-  assumes Y: "corres_choice_true B (\<lbrace>RR\<rbrace> m \<lbrace>\<lambda>rv s. F rv\<rbrace>)"
+  assumes Y: "corres_rv F' dc (\<lambda>_. True) RR (corres_noop) m (\<lambda>_ rv'. F rv')"
+  notes corres_noop_def[simp]
   shows
-  "corres_underlyingK sr nf nf' (corres_choice_false B (\<forall>rv. F rv)) r P (RR and P' and R and (\<lambda>s. \<forall>s'. s = s' \<longrightarrow> PP' s' s)) x (m >>= y)"
+  "corres_underlyingK sr nf nf' F' r P (RR and P' and R and (\<lambda>s. \<forall>s'. s = s' \<longrightarrow> PP' s' s)) x (m >>= y)"
   apply (insert corres)
   apply (simp add: corres_underlyingK_def)
   apply (rule impI)
@@ -711,20 +750,11 @@ lemma corresK_symb_exec_r_search[corres_symb_exec_rs]:
   apply (clarsimp simp: corres_underlying_def corres_underlyingK_def
                         bind_def valid_def empty_fail_def no_fail_def)
   apply (intro impI conjI ballI)
-  apply clarsimp
+    apply clarsimp
     apply (frule(1) use_valid[OF _ X])
-
+    apply (drule corres_rvD[OF Y]; (assumption | simp add: return_def)?)
     apply (frule(1) use_valid[OF _ Z])
-    apply simp
     apply (drule_tac x=aa in meta_spec)
-      apply (cases B)
-       apply (frule(2) use_valid[OF _ Y[THEN corres_choice_trueD]])
-    apply clarsimp
-    apply (drule_tac x="(a, ba)" in bspec,simp)
-    apply (clarsimp)
-    apply (drule(1) bspec)
-    apply clarsimp
-      apply (drule (1) corres_choice_falseD)
     apply clarsimp
     apply (drule_tac x="(a, ba)" in bspec,simp)
     apply (clarsimp)
@@ -732,12 +762,9 @@ lemma corresK_symb_exec_r_search[corres_symb_exec_rs]:
     apply clarsimp
    apply clarsimp
    apply (frule(1) use_valid[OF _ X])
-       apply (frule(1) use_valid[OF _ Z])
-     apply (cases B)
-   apply (frule(2) use_valid[OF _ Y[THEN corres_choice_trueD]])
+   apply (drule corres_rvD[OF Y]; (assumption | simp add: return_def)?)
+   apply (frule(1) use_valid[OF _ Z])
    apply fastforce
-    apply (drule (1) corres_choice_falseD)
-    apply fastforce
   apply (rule no_failD[OF nf],simp+)
   done
 
@@ -799,7 +826,7 @@ lemma corres_stateAssert_implied_frame:
   "corres_underlyingK sr nf nf' (F \<and> F') r (P and P') (Q and Q') f (stateAssert A [] >>= g)"
   apply (clarsimp simp: bind_assoc stateAssert_def)
   apply (corres_search search: C[THEN corresK_unlift])
-  apply (wp | simp add: A)+
+  apply (wp corres_rv_defer | simp add: A)+
   done
 
 lemma corresK_return [corres_concrete_r]:
@@ -866,23 +893,21 @@ lemmas [THEN iffD2, atomized, THEN corresK_lift_rule, rule_format, corresK] =
   corres_liftM2_simp
   corres_liftM_simp
 
-lemma corres_splitEE_str [corres_splits]:
+lemma corresK_splitE [corres_splits]:
   assumes x: "corres_underlyingK sr nf nf' F (f \<oplus> r') P P' a c"
   assumes y: "\<And>rv rv'. corres_protect (r' rv rv') \<Longrightarrow> corres_underlyingK sr nf nf' (F' rv rv') (f \<oplus> r) (R rv) (R' rv') (b rv) (d rv')"
-  assumes z: "\<lbrace>Q\<rbrace> a \<lbrace>R\<rbrace>, \<lbrace>\<lambda>_ _. True\<rbrace>" "\<lbrace>Q'\<rbrace> c \<lbrace>R'\<rbrace>, \<lbrace>\<lambda>_ _. True\<rbrace>"
-  assumes c: "corres_choice_true B (corres_rv sr (\<lambda>(rv :: 'c + 'd) (rv' :: 'e + 'f). (case (rv,rv') of (Inr rva, Inr rva') \<Rightarrow> r' rva rva' \<longrightarrow> F' rva rva' | _ \<Rightarrow> True)) PP PP' a c)"
-  shows      "corres_underlyingK sr nf nf' (F \<and> corres_choice_false B (\<forall>(rv :: 'c + 'd) (rv' :: 'e + 'f). (case (rv,rv') of (Inr rva, Inr rva') \<Rightarrow> r' rva rva' \<longrightarrow> F' rva rva' | _ \<Rightarrow> True))) (f \<oplus> r) (PP and P and Q) (PP' and P' and Q') (a >>=E (\<lambda>rv. b rv)) (c >>=E (\<lambda>rv'. d rv'))"
+  assumes c: "corres_rvE_R F'' r' PP PP' a c F'"
+  assumes z: "\<lbrace>Q\<rbrace> a \<lbrace>R\<rbrace>, -" "\<lbrace>Q'\<rbrace> c \<lbrace>R'\<rbrace>, -"
+  shows      "corres_underlyingK sr nf nf' (F \<and> F'') (f \<oplus> r) (PP and P and Q) (PP' and P' and Q') (a >>=E (\<lambda>rv. b rv)) (c >>=E (\<lambda>rv'. d rv'))"
   unfolding bindE_def
   apply (rule corresK_weakenK)
-  apply (rule corresK_split[OF x, where F'="\<lambda>rv rv'. case (rv,rv') of (Inr rva, Inr rva') \<Rightarrow> F' rva rva' | _ \<Rightarrow> True" and B=B])
+  apply (rule corresK_split[OF x, where F'="\<lambda>rv rv'. case (rv,rv') of (Inr rva, Inr rva') \<Rightarrow> F' rva rva' | _ \<Rightarrow> True"])
   apply (simp add: corres_protect_def)
-    prefer 4
-    apply (cases B)
+    prefer 2
     apply simp
-    apply (rule corres_rv_weaken[OF _ c[THEN corres_choice_trueD]])
+    apply (rule corres_rv_prove[where F=F''])
     apply (case_tac rv; case_tac rv'; simp)
-    apply simp
-    apply simp
+    apply (rule corres_rvE_RD[OF c]; assumption)
     apply (case_tac rv; case_tac rv'; simp)
      apply (simp add: corres_underlyingK_def corres_protect_def)
     apply (rule corresK_weaken)
@@ -897,7 +922,7 @@ lemma corres_splitEE_str [corres_splits]:
                         | _ \<Rightarrow> True)"; assumption?)
       apply clarsimp+
    apply (insert z)
-  by ((fastforce simp: valid_def validE_def split: sum.splits)+)
+  by ((fastforce simp: valid_def validE_def validE_R_def split: sum.splits)+)
 
 lemma corresK_returnOk [corres_concrete_r]:
   "corres_underlyingK sr nf nf' (r (Inr a) (Inr b)) r \<top> \<top> (returnOk a) (returnOk b)"
@@ -928,6 +953,8 @@ lemma corresK_fail_no_fail'[corresK]:
   by (fastforce intro!: corres_fail)
 
 
+
+
 (* Wrap it up in a big hammer. Small optimization to avoid searching when no fact is given. *)
 
 named_theorems correswp_wp_comb and correswp_wp_comb_del
@@ -937,26 +964,16 @@ lemma corres_inst_eq_imp:
 
 lemmas corres_hoare_pre = hoare_pre[# \<open>-\<close> \<open>atomize (full), rule allI, rule corres_inst_eq_imp\<close>]
 
-named_theorems correswp
-
-lemmas [correswp] =
-  corres_choice_rv_defer_no_args
-
-method correswp_once uses wp =
+method correswp uses wp =
   (determ \<open>
-     corres_inst
-   | (fails \<open>schematic_hoare_pre\<close>, (wp_once add: correswp wp))
+     (fails \<open>schematic_hoare_pre\<close>, (wp add: wp))
    | (schematic_hoare_pre,
         (use correswp_wp_comb [wp_comb]
              correswp_wp_comb_del[wp_comb del]
              hoare_pre[wp_pre del]
              corres_hoare_pre[wp_pre]
         in
-      \<open>use in \<open>wp_once add: correswp wp\<close>\<close>))\<close>;
-    (fails \<open>rule TrueI\<close>, rule corres_inst_eqI)?)
-
-method correswp uses wp =
-  ((correswp_once wp: wp)+)[1]
+      \<open>use in \<open>wp add: wp\<close>\<close>))\<close>)
 
 lemmas [correswp_wp_comb_del] =
   hoare_vcg_precond_imp
@@ -965,16 +982,24 @@ lemmas [correswp_wp_comb_del] =
   hoare_wp_state_combsE(1)
   hoare_wp_state_combsE(2)
 
-lemmas [correswp_wp_comb] =
-  correswp_wp_comb_del[# \<open>-\<close> \<open>atomize (full), rule allI, rule corres_inst_eq_imp\<close>]
-
-declare hoare_post_comb_imp_conj[correswp_wp_comb_del]
-
 lemma corres_inst_conj_lift[correswp_wp_comb]:
   "\<lbrakk>\<lbrace>R\<rbrace> f \<lbrace>Q\<rbrace>; \<lbrace>P'\<rbrace> f \<lbrace>Q'\<rbrace>; \<And>s. corres_inst_eq (R s) (P s)\<rbrakk> \<Longrightarrow>
        \<lbrace>\<lambda>s. P s \<and> P' s\<rbrace> f \<lbrace>\<lambda>rv s. Q rv s \<and> Q' rv s\<rbrace>"
   by (rule hoare_vcg_conj_lift; simp add: valid_def corres_inst_eq_def)
 
+lemmas [correswp_wp_comb] =
+  correswp_wp_comb_del[# \<open>-\<close> \<open>atomize (full), rule allI, rule corres_inst_eq_imp\<close>]
+  valid_validE_R
+  hoare_vcg_R_conj[OF valid_validE_R]
+  hoare_vcg_E_elim[OF valid_validE_E]
+  hoare_vcg_E_conj[OF valid_validE_E]
+  validE_validE_R
+  hoare_vcg_R_conj
+  hoare_vcg_E_elim
+  hoare_vcg_E_conj
+  hoare_vcg_conj_lift
+
+declare hoare_post_comb_imp_conj[correswp_wp_comb_del]
 
 method corressimp uses simp cong search wp
   declares corres corresK corres_splits corresc_simp =
@@ -1064,14 +1089,17 @@ experiment
   begin
 
   lemmas f_Q' = f_corres[atomized, @\<open>use_corres frame: frameA\<close>]
+
   lemma "G \<Longrightarrow> F \<Longrightarrow> corres_underlying sr False True dc (P and PP) (P' and PP')
     (g >>= (K (f >>= K (assert True)))) (g' >>= (K (f' >>= (\<lambda>rv'. (stateAssert (QQ' rv') [])))))"
   apply (simp only: stateAssert_def K_def)
   apply corres
   apply (corres_search search: corresK_assert)
+  apply (correswp)+
+  apply corres_rv
   apply (correswp wp: f_Q' | simp)+
   apply corres
-  apply (wp | simp)+
+  apply (correswp | simp)+
   by auto
 
 end
